cub now separates in and out arguments
started cub arg refactor

rebasing changes from main

rebasing shift and lifting updates

rebasing removing infer member types

refactoring

updating shift and lift changes

working on new copy in copy out

rebasing with lifting updates

new copyin copyout in big step

editing big step properties proofs

rebasing shifting and lifting updates

editing lemmas

rebasing for set header validity

rebasing for shifting lifting updates

inn out map lemmas

rebasing shifting lifting changes

attempting to prove table case in shift eval

edited lifted proofs

edits

proved one shift stm lemma

another shifting proof for stms

statement shifting lemmas proven

started refactoring interpreter

interpreter refactored

fixed to p4cub

gcl builds

builds

lib/printp4cub.ml
@@ -55,11 +55,8 @@ let print_bin p b =
   in
   fprintf p "%s" s
 
-let print_paramarg printa printb p (ab : ('a,'b) paramarg) = 
-  match ab with
-  | PAIn a -> fprintf p "PAIn <%a>" printa a
-  | PAOut b -> fprintf p "PAOut <%a>" printb b
-  | PAInOut b -> fprintf p "PAInOut <%a>" printb b
+let print_inout printa printb p ({inn; out} : ('a,'b) InOut.t) =
+ fprintf p "@[inn: <%a>, out: <%a>@]" printa inn printb out
 
 let print_list ?(sep="") f p l =
   let print_item b x =
@@ -82,10 +79,10 @@ let print_fields print1 print2 p (f : ('a * 'b) list) =
   else ()
 
 
-let print_arrow printk printa printb p (ar: ('k,'a,'b) arrow) =
+let print_arrow printk printa printb p (ar: ('k,'a,'b) Arr.t) =
   fprintf p "@[paramargs: <%a>, rtrns: <%a>@]"
-    (print_fields printk (print_paramarg printa printb)) ar.paramargs
-    (print_option printb) ar.rtrns 
+    (print_inout printk printa) ar.inout
+    (print_option printb) ar.ret
 
 
 let print_string_string_field =
@@ -114,10 +111,9 @@ let rec print_type p (t:Typ.t) =
                                   print_bigint l  
   | Typ.Var n -> fprintf p "TVar <%a>" my_print_int n
 
-let print_params p (pa: Typ.params) = 
-  print_fields print_string (print_paramarg print_type print_type) p pa
+let print_params = print_inout (print_fields print_string print_type) (print_fields print_string print_type)
 
-let print_arrowT = print_arrow print_string print_type print_type
+let print_arrowT = print_arrow (print_fields print_string print_type) (print_fields print_string print_type) print_type
 
 let print_ct p = 
   function
@@ -193,8 +189,7 @@ let rec print_exp p =
         print_exp e2
 
 
-let print_args p (a : Exp.args) =
-  (print_list ~sep:"," (print_paramarg print_exp print_exp)) p a
+let print_args = print_inout (print_list ~sep:"," print_exp) (print_list ~sep:"," print_exp)
 
 let print_constructor_args p (c : Top.constructor_args) =
   (print_list ~sep:"," print_string) p c
